src/Actus/Compiler.lean
@@ -1,0 +1,110 @@
+import Actus.Logic
+import Actus.Automata
+
+open MetricTemporal TimedFinite
+variable {T : Type} [AtomicProp T]
+
+def Proposition.nnf (p : Proposition T) : Proposition T :=
+  match p with
+  | mtt => mtt
+  | [[x]] => [[x]]
+  | ~ φ' =>
+    match φ' with
+    | mtt => mtf
+    | [[x]] => ~ [[x]]
+    | ~ φ'' => nnf φ''
+    | φ and ψ => (nnf (~ φ)) or (nnf (~ ψ))
+    | φ U ψ in w => (nnf (~ φ)) S (nnf (~ ψ)) in w
+    | φ S ψ in w => (nnf (~ φ)) U (nnf (~ ψ)) in w
+  | φ and ψ => (nnf φ) and (nnf ψ)
+  | φ U ψ in w => (nnf φ) U (nnf ψ) in w
+  | φ S ψ in w => (nnf φ) S (nnf ψ) in w
+
+namespace NnfCorrect
+  theorem doubleNegationCorrect (φ : Proposition T) : MetricTemporalSemantics.equiv φ (~ (~ φ)) := by
+    unfold MetricTemporalSemantics.equiv <;> intros
+    apply Iff.intro <;> intro H
+    . sorry
+    . sorry
+  -- lemma for demorgan.
+  theorem nnfCorrect (φ : Proposition T) : MetricTemporalSemantics.equiv φ (Proposition.nnf φ) := by
+    unfold MetricTemporalSemantics.equiv <;> intros
+    sorry
+end NnfCorrect
+
+inductive TableauNode (T : Type) where
+| leaf : Proposition T -> TableauNode T
+| and : TableauNode T -> TableauNode T -> TableauNode T
+| or : TableauNode T -> TableauNode T -> TableauNode T
+| until : TableauNode T -> Window -> TableauNode T -> TableauNode T
+| since : TableauNode T -> Window -> TableauNode T -> TableauNode T
+
+def Proposition.toTableau {T : Type} (φ : Proposition T) : TableauNode T :=
+  let rec toTableauRec (ψ : Proposition T) : TableauNode T :=
+    match ψ with
+    | mtt => .leaf mtt
+    | [[x]] => .leaf [[x]]
+    | ~ [[x]] => .leaf (~ [[x]])
+    | φ' and ψ' => .and (toTableauRec φ') (toTableauRec ψ')
+    | φ' U ψ' in w => .until (toTableauRec φ') w (toTableauRec ψ')
+    | φ' S ψ' in w => .since (toTableauRec φ') w (toTableauRec ψ')
+    | ~ (φ' and ψ') => .or (toTableauRec (~ φ')) (toTableauRec (~ ψ'))
+    | _ => .leaf ψ -- Should be unreachable due to nnf correctness
+  toTableauRec (nnf φ)
+
+def TableauNode.collectAtomicProps : TableauNode T -> Lean.HashSet T
+| .leaf p => p.collectAtomicProps
+| .and n1 n2 => n1.collectAtomicProps.merge n2.collectAtomicProps
+| .or n1 n2 => n1.collectAtomicProps.merge n2.collectAtomicProps
+| .until n1 _ n2 => n1.collectAtomicProps.merge n2.collectAtomicProps
+| .since n1 _ n2 => n1.collectAtomicProps.merge n2.collectAtomicProps
+
+namespace Beta
+--   def TableauNode.toTfa (node : TableauNode T) : TFA T :=
+--   let rec build (node' : TableauNode T) (stateCounter : Nat) (clockCounter : Nat) : (TFA T × State × Nat × Nat) :=
+--       match node' with
+--       | .leaf p =>
+--       let state := { idx := stateCounter }
+--       let states := Lean.HashSet.empty.insert state
+--       let tfa := {
+--           states,
+--           alphabet := Lean.HashSet.empty.insert p
+--           initialState := state,
+--           acceptingStates := states,
+--           transitions := [],
+--       }
+--       (tfa, state, stateCounter + 1, clockCounter)
+--       | .and n1 n2 =>
+--       let (tfa1, s1, sc1, cc1) := build n1 stateCounter clockCounter
+--       let (tfa2, s2, sc2, cc2) := build n2 sc1 cc1
+--       let newState := { idx := sc2 }
+--       let tfa := {
+--           states := tfa1.states.insert newState,
+--           alphabet := tfa1.alphabet.merge tfa2.alphabet,
+--           initialState := newState,
+--           transitions := tfa1.transitions ++ tfa2.transitions ++ [
+--           { source := newState, target := s1, symbol := mtt, guard := { clock := ⟨cc2⟩, op := .le, bound := 0 }, reset := [] },
+--           { source := newState, target := s2, symbol := mtt, guard := { clock := ⟨cc2⟩, op := .le, bound := 0 }, reset := [] }
+--           ],
+--           acceptingStates := tfa1.acceptingStates.merge tfa2.acceptingStates
+--       }
+--       (tfa, newState, sc2 + 1, cc2 + 1)
+--       | .or n1 n2 =>
+--       let (tfa1, s1, sc1, cc1) := build n1 stateCounter clockCounter
+--       let (tfa2, s2, sc2, cc2) := build n2 sc1 cc1
+--       let newState := { idx := sc2 }
+--       let tfa := {
+--           states := tfa1.states.insert newState,
+--           alphabet := tfa1.alphabet.merge tfa2.alphabet,
+--           initialState := newState,
+--           transitions := tfa1.transitions ++ tfa2.transitions ++ [
+--           { source := newState, target := s1, symbol := mtt, guard := { clock := ⟨cc2⟩, op := .le, bound := 0 }, reset := [] },
+--           { source := newState, target := s2, symbol := mtt, guard := { clock := ⟨cc2⟩, op := .le, bound := 0 }, reset := [] }
+--           ],
+--           acceptingStates := tfa1.acceptingStates.merge tfa2.acceptingStates
+--       }
+--       (tfa, newState, sc2 + 1, cc2 + 1)
+--       | .until n1 w n2 => sorry
+--       | .since n1 w n2 => sorry
+--   build node 0 0
+end Beta
